

19-20

$$1. P: P(A_1) \cdot \left[ 1 - \left[ 1 - P(B_1)P(B_2) \right] \left[ 1 - P(C_1) \right] \left[ 1 - P(C_2) \right] \right] \cdot P(A_2) = 0.798984$$

$$2. 1) P = P(Z_1=0) + P(Z_1=0, Z_2=1) + P(Z_{21}=0, Z_{22}=0, Z_1=2)$$

$$= \frac{1}{4} + \frac{1}{2} \cdot \frac{1}{4} + \frac{1}{4} \cdot \frac{1}{4} \cdot \frac{1}{4} = \frac{25}{64}$$

$$2) P = P(Z_{21}=2, Z_{22}=2, Z_1=2) = \frac{1}{4} \cdot \frac{1}{4} \cdot \frac{1}{4} = \frac{1}{64}$$

$$\begin{aligned} 3. P(X_1 < X_2 < X_3) &= \sum_{i=1}^{\infty} (1-P_1) P_1^{i-1} \sum_{j=i+1}^{\infty} (1-P_2) P_2^{j-1} \sum_{k=j+1}^{\infty} (1-P_3) P_3^{k-1} \\ &= \sum_{i=1}^{\infty} (1-P_1) P_1^{i-1} \sum_{j=i+1}^{\infty} (1-P_2) P_3 (P_2 P_3)^{j-1} = \sum_{i=1}^{\infty} (1-P_1) P_1^{i-1} \frac{(1-P_2) P_3 (P_2 P_3)^i}{1-P_2 P_3} \\ &= \frac{(1-P_1)(1-P_2) P_2 P_3^2}{(1-P_2 P_3)(1-P_1 P_2 P_3)} \end{aligned}$$

$$4. 1) \text{ 设 } W_3 = \xi_1 + \xi_2 + \xi_3 \quad \text{则} \quad \begin{aligned} \xi_1 &= W_1 W_3 \\ \xi_2 &= (W_2 - W_1) W_3 \\ \xi_3 &= W_3 - W_2 W_3 \end{aligned} \quad \int_{-1}^1 \frac{1}{2} x^4 dx = \frac{2}{5}$$

$$\frac{\partial(\xi_1, \xi_2, \xi_3)}{\partial(W_1, W_2, W_3)} = W_3^2$$

$$\begin{aligned} \therefore P(W_1, W_2, W_3) &= e^{-W_1 W_3} \cdot e^{-(W_2 - W_1) W_3} \cdot e^{-(W_3 - W_2 W_3)} \cdot W_3^2 \\ &= e^{-W_3} W_3^2 \end{aligned} \quad \frac{1}{5} - \frac{1}{9}$$

$$\text{又 } P(W_1, W_2) = \int_0^{+\infty} e^{-W_3} W_3^2 dW_3 = 2 \quad (0 < W_1 < W_2 < 1)$$

$$2) \because P(0 < W_2 < \frac{1}{2}, \frac{1}{2} < W_1 < 1) = 0$$

而  $P(0 < W_2 < \frac{1}{2})$ ,  $P(\frac{1}{2} < W_1 < 1)$  显然不为 0 故不独立

$$5. D(U+V) = D(3\xi - 3\eta) = 9[Var(\xi) + Var(\eta) - 2Cov(\xi, \eta)]$$

$$\because \xi, \eta \text{ 独立} \quad Var(\xi) = Var(\eta) = \frac{1}{3} \quad \therefore D(U+V) = 6$$

$$D(U^2+V^2) = D(5(\xi^2 + \eta^2)) = 25[Var(\xi^2) + Var(\eta^2)] = \frac{40}{9}$$

$$Var(\xi^2) = E(\xi^4) - E^2(\xi^2) = \frac{1}{5} - \frac{1}{9} = \frac{4}{45}$$

6. ?

7. 由泊松分布的可加性 记  $\sum_{i=1}^n \lambda_i = m$  则  $\frac{\xi_1 + \dots + \xi_n}{\lambda_1 + \dots + \lambda_n} \sim \frac{P(m)}{m}$

则  $\frac{P(m)}{m}$  的特征函数为  $f_{P(m)}(\frac{t}{m}) = e^{m(e^{i\frac{t}{m}} - 1)}$   $\because m \rightarrow +\infty$

$$\therefore e^{m(e^{i\frac{t}{m}} - 1)} = e^{m(i\frac{t}{m} + o(\frac{t}{m}))} \rightarrow e^{it}$$

而  $e^{it}$  为 1 的特征函数 由特征函数的唯一性可知  $\frac{\xi_1 + \dots + \xi_n}{\lambda_1 + \dots + \lambda_n} \xrightarrow{d} 1$

等价于  $\frac{\xi_1 + \dots + \xi_n}{\lambda_1 + \dots + \lambda_n} \xrightarrow{P} 1$